StrataTest/Languages/Core/Examples/Functions.lean
@@ -3,12 +3,13 @@
 
   SPDX-License-Identifier: Apache-2.0 OR MIT
 -/
+module
 
-import Strata.Languages.Core
-import Strata.Languages.Core.CallGraph
+meta import Strata.Languages.Core
+meta import Strata.Languages.Core.CallGraph
 import StrataDDM.Integration.Lean.HashCommands
-import Strata.MetaVerifier
 
+meta section
 open StrataDDM (Program)
 ---------------------------------------------------------------------
 namespace Strata
@@ -74,10 +75,6 @@ Result: ✅ pass
 -/
 #guard_msgs in
 #eval Core.verify funcPgm
-
-theorem funcPgm_correct : smtVCsCorrect funcPgm := by
-  gen_smt_vcs
-  all_goals (try grind)
 
 ---------------------------------------------------------------------
 
@@ -158,9 +155,6 @@ Result: ✅ pass
 #guard_msgs in
 #eval Core.verify quantBodyFuncPgm
 
-theorem quantBodyFuncPgm_correct : smtVCsCorrect quantBodyFuncPgm := by
-  gen_smt_vcs
-  all_goals (try grind)
-
 end Strata
+end
 ---------------------------------------------------------------------
