StrataTest/Languages/Core/Examples/Min.lean
@@ -3,11 +3,12 @@
 
   SPDX-License-Identifier: Apache-2.0 OR MIT
 -/
+module
 
-import Strata.Languages.Core
+meta import Strata.Languages.Core
 import StrataDDM.Integration.Lean.HashCommands
-import Strata.MetaVerifier
 
+meta section
 open StrataDDM (Program)
 ---------------------------------------------------------------------
 namespace Strata
@@ -46,9 +47,6 @@ Result: ✅ pass
 #guard_msgs in
 #eval Core.verify testPgm
 
-theorem testPgm_correct : smtVCsCorrect testPgm := by
-  gen_smt_vcs
-  grind
-
 end Strata
+end
 ---------------------------------------------------------------------
