StrataTest/Languages/Core/Examples/Quantifiers.lean
@@ -3,11 +3,12 @@
 
   SPDX-License-Identifier: Apache-2.0 OR MIT
 -/
+module
 
-import Strata.Languages.Core
+meta import Strata.Languages.Core
 import StrataDDM.Integration.Lean.HashCommands
-import Strata.MetaVerifier
 
+meta section
 ---------------------------------------------------------------------
 namespace Strata
 
@@ -151,8 +152,5 @@ Result: ✅ pass
 #guard_msgs in
 #eval Core.verify triggerPgm
 
-theorem triggerPgm_correct : smtVCsCorrect triggerPgm := by
-  gen_smt_vcs
-  all_goals (try grind)
-
 end Strata
+end
